{-# OPTIONS --rewriting #-}

open import Agda.Primitive using (Level;lsuc;_⊔_;lzero)
open import Lib
open import Interval
open import Path
open import Equiv
open import Proposition
open import Cofibs
open import Kan
open import Glue

module Glue-Weak where

  private
    -- this stronger version is true, but doesn't get used for wcoe
    glue-weak-and-β : ∀ {l} {α : Set} {{_ : Cofib α}} {T : α → Set l} {B : Set l} {f : (u : α) → T u → B}
                      → hasHCom B
                      → (b : B) 
                      → (t : (pα : α) → HFiber (f pα) b)
                      → (HFiber {A = (Glue α T B f)} {B} unglue b) [ α ↦ (\ pα → HFiber-unglue-α _ pα (t pα)) ]
    glue-weak-and-β {α = α} {{ cα }}{T} hcomB b t = 
                          (glue _ _ _ _ 
                               (\ pα → fst (t pα))
                               (fst (fill `0) , (\ pα → fst (snd (fill `0)) pα ∘ ! (fst (snd (snd (t pα)))))),
                           (((\ z → fst (fill z)) , id , ! (snd (snd (fill `1)) id)) 
                            ∘= Glueβ _ _)) , 
                          (λ pα → =HFiber 
                                  (glue-cong _ _ _ _ _ _ (λ= \ pα' → apd (\ x → fst (t x)) (Cofib.eq cα pα pα')  ) (fst (snd (fill `0)) pα ∘ ! (fst (snd (snd (t pα))))) ∘ Glue-α-! _ _)
                                  (λ= (\ x → fst (snd (hcomB `1 x α (λ x₁ pα₁ → fst (snd (t pα₁)) x₁) (b , (λ pα₁ → snd (snd (snd (t pα₁))))))) pα))) where
       fill : (z : _) → _
       fill z = hcomB `1 z α (\ x pα → fst (snd (t pα)) x) 
                             (b , (λ pα → snd (snd (snd (t pα))) ))

  glue-weak : ∀ {l} {α : Set} {{cα : Cofib α}} {T : α → Set l} {B : Set l} {f : (u : α) → T u → B}
            → hasHCom B
            → (b : B) 
            → (t : (pα : α) → HFiber (f pα) b)
            → (Glue α T B f)
  glue-weak {α = α} {{ cα }}{T} hcomB b t =
       glue _ _ _ _ 
           (\ pα → fst (t pα))
           (fst fix , (\ pα → fst (snd fix) pα ∘ ! (fst (snd (snd (t pα)))))) where
       fix = hcomB `1 `0
                   α (\ x pα → fst (snd (t pα)) x) 
                   (b , (λ pα → snd (snd (snd (t pα))) ))

  glue-weak-α : ∀ {l} {α : Set} {{_ : Cofib α}} {T : α → Set l} {B : Set l} {f : (u : α) → T u → B}
            → (hcomB : hasHCom B)
            → (b : B) 
            → (t : (pα : α) → HFiber (f pα) b)
            → (pα : α) → coe (Glue-α α T B f pα) (glue-weak hcomB b t) == fst (t pα)
  glue-weak-α hcomB b t pα = glue-α _ _ _

  Glue-to-fiber : ∀ {l} {α : Set} {{cα : Cofib α}} {T : α → Set l} {B : Set l} {f : (u : α) → T u → B}
                    → (g : Glue α T B f)
                    → ((pα : α) → HFiber (f pα) (unglue g))
  Glue-to-fiber g = (\ pα → (coe (Glue-α _ _ _ _ pα) g ) , (\ _ → unglue g) , ! (unglue-α g pα) , id ) 

  -- could also show that the weak β is path-equal to refl, but don't need that below?
  glue-weak-η : ∀ {l} {α : Set} {{cα : Cofib α}} {T : α → Set l} {B : Set l} {f : (u : α) → T u → B}
              → (hb : hasHCom B)
              → (g : Glue α T B f)
              → Path (Glue α T B f)
                      (glue-weak {α = α} {{cα}}{T}{B}{f} hb (unglue g) (Glue-to-fiber g))
                      g 
  glue-weak-η {α = α} hcomB g = 
    (! (Glueη _) =∘ ((\ x → glue _ _ _ _ (\ pα → fst (Glue-to-fiber g pα)) 
                                         (fst (fillB x) , 
                                          (\ pα → fst (snd (fillB x)) pα ∘ unglue-α g pα))) , 
                    (ap (glue _ _ _ _ _) (pair= id (λ= \ _ → uip))) , 
                    (ap (glue _ _ _ _ _) (pair= (! (snd (snd (fillB `1)) id)) (λ= \ _ → uip))))) where
    fillB : (x : _) → _
    fillB x = (hcomB `1 x α (λ x pα → unglue g) (unglue g , (λ pα → id)))

  glue-weak= : ∀ {l} {α : Set} {{_ : Cofib α}} {T : α → Set l} {B : Set l} {f : (u : α) → T u → B}
              → (hcomB : hasHCom B)
              → (b b' : B) 
              → (t : (pα : α) → HFiber (f pα) b)
              → (t' : (pα : α) → HFiber (f pα) b')
              → b == b'
              → ((pα : α) → t pα =h t' pα)
              → glue-weak hcomB b t == glue-weak hcomB b' t'
  glue-weak= hcomB b b' t t' id h = ap {M = t} {N = t'} (glue-weak hcomB b) (λ= \ pα → het-to-hom (h pα))



  -- repackaging of CCHM final steps
  -- note: this is *almost* rearrangeable into
  --       unglue, glue-to-fiber : Glue α T B f ≃ Σ (x : B). α → HFiber f b
  -- but the equality is strict in the input
  -- and not proved in the output (though it looks like it would be weak)

  glue-weak-better : ∀ {l} {α : Set} {{cα : Cofib α}} {T : α → Set l} {B : Set l} {f : (u : α) → T u → B}
                   → hasHCom B
                   → (β : Set) {{cβ : Cofib β}}
                   → (g : β → (Glue α T B f)) -- already have a partial answer
                   → (b : B [ β ↦ (\ pβ → unglue (g pβ)) ]) 
                   → (t : (pα : α) → HFiber (f pα) (fst b)
                       [ β ↦ (\ pβ → transport (HFiber (f pα))
                                               (snd b pβ)
                                               (Glue-to-fiber (g pβ) pα)) ])
                   → (Glue α T B f) [ β ↦ g ]
  glue-weak-better {α = α} {{ cα }} {T} {f = f} hcomB β g b t =
      g' , (\ pβ → glue-cong _ _ _ _ _ _ (λ= \ pα → ap fst (snd (t pα) pβ) ∘ ! (fst-transport-HFiber-base (f pα) (snd b pβ) (Glue-to-fiber (g pβ) pα)))
                                         (fst (snd fix) (inr pβ)) ∘ Glueη (g pβ)) where
       fix = hcomB `1 `0
                      (α ∨ β)
                      (\ x → case (\ pα →  fst (snd (fst (t pα))) x )
                                  (\ pβ → unglue (g pβ))
                                  (\ pα pβ →  ap= (fst-snd-transport-HFiber-base (f pα) (snd b pβ) (Glue-to-fiber (g pβ) pα))
                                              ∘ ! (ap (\ H → fst (snd H) x) (snd (t pα) pβ)))) 
                      (fst b ,  ∨-elim _
                                       (\ pα → snd (snd (snd (fst (t pα)))) )
                                       (\ pβ → snd b pβ)
                                       (\ _ _ → uip)  )

       g' = glue _ _ _ _ (\ pα →  fst (fst (t pα)) )
                         (fst fix ,
                          (\ pα → fst (snd fix) (inl pα) ∘ ! (fst (snd (snd (fst (t pα)))))))

  -- this version makes the η definitional if you specify up front that you want it
  glue-weak-better-η : ∀ {l} {α : Set} {{cα : Cofib α}} {T : α → Set l} {B : Set l} {f : (u : α) → T u → B}
                     → (hb : hasHCom B)
                     → (g : Glue α T B f)
                     → fst (glue-weak-better {α = α} {{cα}}{T}{B}{f} hb (`0 == `0) (\ _ → g) (unglue g , (\ _ → id)) (\ pα → (Glue-to-fiber g pα , (\ _ → id))))
                       == g
  glue-weak-better-η hb g = ! (snd (glue-weak-better hb (`0 == `0) (\ _ → g) (unglue g , (\ _ → id)) (\ pα → (Glue-to-fiber g pα , (\ _ → id)))) id)


  Glue-to-fiber' : ∀ {l} {α : Set} {{cα : Cofib α}} {T : α → Set l} {B : Set l} {f : (u : α) → T u → B}
                    → (g : Glue α T B f)
                    → ((pα : α) → HFiber' (f pα) (unglue g))
  Glue-to-fiber' g = (\ pα → (coe (Glue-α _ _ _ _ pα) g ) , (\ _ → unglue g) , id , ! (unglue-α g pα) ) 

  -- hcom in other direction for flipped hfiber
  glue-weak-better' : ∀ {l} {α : Set} {{cα : Cofib α}} {T : α → Set l} {B : Set l} {f : (u : α) → T u → B}
                   → hasHCom B
                   → (β : Set) {{cβ : Cofib β}}
                   → (g : β → (Glue α T B f)) -- already have a partial answer
                   → (b : B [ β ↦ (\ pβ → unglue (g pβ)) ]) 
                   → (t : (pα : α) → HFiber' (f pα) (fst b)
                       [ β ↦ (\ pβ → transport (HFiber' (f pα)) (snd b pβ)
                                               (Glue-to-fiber' (g pβ) pα)) ])
                   → (Glue α T B f) [ β ↦ g ]
  glue-weak-better' {α = α} {{ cα }} {T} {f = f} hcomB β g b t =
    g' ,
    ((\ pβ → glue-cong _ _ _ _ _ _ (λ= \ pα → ap fst (snd (t pα) pβ) ∘ ! (fst-transport-HFiber'-base (f pα) (snd b pβ) (Glue-to-fiber' (g pβ) pα))) (fst (snd fix) (inr pβ)) ∘ Glueη (g pβ))) where
      fix = hcomB `0 `1
                   (α ∨ β)
                   (\ x → case (\ pα →  fst (snd (fst (t pα))) x )
                               (\ pβ → unglue (g pβ))
                               (\ pα pβ →   ap= (fst-snd-transport-HFiber'-base (f pα) (snd b pβ) (Glue-to-fiber' (g pβ) pα))
                                           ∘  ! (ap (\ H → fst (snd H) x) (snd (t pα) pβ)) )) 
                        (fst b ,  ∨-elim _
                                         (\ pα →  fst (snd (snd (fst (t pα))))  )
                                         (\ pβ → snd b pβ)
                                         (\ _ _ → uip)  )
      
      g' = glue _ _ _ _ (\ pα →  fst (fst (t pα)) )
                        (fst fix ,
                         (\ pα → fst (snd fix) (inl pα) ∘ ! (snd (snd (snd (fst (t pα)))))))
